Stardardised diff_inv

HS_ODEs.thy
@@ -98,19 +98,19 @@ no_notation g_orbit ("\<gamma>")
 
 subsection \<open> Differential Invariants \<close>
 
-definition diff_inv :: "('a \<Rightarrow> bool) \<Rightarrow> (real \<Rightarrow> ('a::real_normed_vector) \<Rightarrow> 'a) \<Rightarrow> 
-  ('a \<Rightarrow> real set) \<Rightarrow> 'a set \<Rightarrow> real \<Rightarrow> ('a \<Rightarrow> bool) \<Rightarrow> bool" 
-  where "diff_inv I f U S t\<^sub>0 G \<equiv> (\<Union> \<circ> (\<P> (g_orbital f G U S t\<^sub>0))) {s. I s} \<subseteq> {s. I s}"
+definition diff_inv :: "('a \<Rightarrow> real set) \<Rightarrow> 'a set \<Rightarrow> ('a \<Rightarrow> bool) 
+  \<Rightarrow> (real \<Rightarrow> ('a::real_normed_vector) \<Rightarrow> 'a) \<Rightarrow> real \<Rightarrow> ('a \<Rightarrow> bool) \<Rightarrow> bool" 
+  where "diff_inv U S G f t\<^sub>0 I \<equiv> (\<Union> \<circ> (\<P> (g_orbital f G U S t\<^sub>0))) {s. I s} \<subseteq> {s. I s}"
 
-lemma diff_inv_eq: "diff_inv I f U S t\<^sub>0 G = 
+lemma diff_inv_eq: "diff_inv U S G f t\<^sub>0 I = 
   (\<forall>s. I s \<longrightarrow> (\<forall>X\<in>Sols U S f t\<^sub>0 s. (\<forall>t\<in>U s.(\<forall>\<tau>\<in>(down (U s) t). G (X \<tau>)) \<longrightarrow> I (X t))))"
   unfolding diff_inv_def g_orbital_eq image_le_pred by auto
 
 lemma diff_inv_eq_inv_set:
-  "diff_inv I f U S t\<^sub>0 G = (\<forall>s. I s \<longrightarrow> (g_orbital f G U S t\<^sub>0 s) \<subseteq> {s. I s})"
+  "diff_inv U S G f t\<^sub>0 I = (\<forall>s. I s \<longrightarrow> (g_orbital f G U S t\<^sub>0 s) \<subseteq> {s. I s})"
   unfolding diff_inv_eq g_orbital_eq image_le_pred by auto
 
-lemma "diff_inv I f U S t\<^sub>0 (\<lambda>s. True) \<Longrightarrow> diff_inv I f U S t\<^sub>0 G"
+lemma "diff_inv U S (\<lambda>s. True) f t\<^sub>0 I \<Longrightarrow> diff_inv U S G f t\<^sub>0 I"
   unfolding diff_inv_eq by auto
 
 named_theorems diff_inv_rules "rules for certifying differential invariants"
@@ -120,7 +120,7 @@ lemma diff_inv_eq_rule [diff_inv_rules]:
   assumes Uhyp: "\<And>s. s \<in> S \<Longrightarrow> is_interval (U s)"
     and dX: "\<And>X t. (D X = (\<lambda>\<tau>. f \<tau> (X \<tau>)) on U(X t\<^sub>0)) \<Longrightarrow> 
   \<forall>\<tau>\<in>(down (U(X t\<^sub>0)) t). G (X \<tau>) \<Longrightarrow> D (\<lambda>\<tau>. \<mu> (X \<tau>) - \<nu> (X \<tau>)) = (\<lambda>\<tau>. \<tau> *\<^sub>R 0) on U(X t\<^sub>0)"
-  shows "diff_inv (\<lambda>s. \<mu> s = \<nu> s) f U S t\<^sub>0 G"
+  shows "diff_inv U S G f t\<^sub>0 (\<lambda>s. \<mu> s = \<nu> s)"
 proof(simp add: diff_inv_eq ivp_sols_def, clarsimp)
   fix X t 
   assume xivp:"D X = (\<lambda>\<tau>. f \<tau> (X \<tau>)) on U (X t\<^sub>0)" "\<mu> (X t\<^sub>0) = \<nu> (X t\<^sub>0)" "X \<in> U (X t\<^sub>0) \<rightarrow> S"
@@ -141,7 +141,7 @@ lemma diff_inv_eq_rule_old:
   fixes \<mu>::"'a::banach \<Rightarrow> real"
   assumes Uhyp: "\<And>s. s \<in> S \<Longrightarrow> is_interval (U s)"
     and dX: "\<And>X. (D X = (\<lambda>\<tau>. f \<tau> (X \<tau>)) on U(X t\<^sub>0)) \<Longrightarrow> (D (\<lambda>\<tau>. \<mu>(X \<tau>)-\<nu>(X \<tau>)) = ((*\<^sub>R) 0) on U(X t\<^sub>0))"
-  shows "diff_inv (\<lambda>s. \<mu> s = \<nu> s) f U S t\<^sub>0 G"
+  shows "diff_inv U S G f t\<^sub>0 (\<lambda>s. \<mu> s = \<nu> s)"
   apply(rule diff_inv_eq_rule[OF Uhyp], simp)
   by (frule dX, simp)
 
@@ -151,7 +151,7 @@ lemma diff_inv_leq_rule [diff_inv_rules]:
     and Gg: "\<And>X. (D X = (\<lambda>\<tau>. f \<tau> (X \<tau>)) on U(X t\<^sub>0)) \<Longrightarrow> (\<forall>\<tau>\<in>U(X t\<^sub>0). \<tau> > t\<^sub>0 \<longrightarrow> G (X \<tau>) \<longrightarrow> \<mu>' (X \<tau>) \<ge> \<nu>' (X \<tau>))"
     and Gl: "\<And>X. (D X = (\<lambda>\<tau>. f \<tau> (X \<tau>)) on U(X t\<^sub>0)) \<Longrightarrow> (\<forall>\<tau>\<in>U(X t\<^sub>0). \<tau> < t\<^sub>0 \<longrightarrow> \<mu>' (X \<tau>) \<le> \<nu>' (X \<tau>))"
     and dX: "\<And>X. (D X = (\<lambda>\<tau>. f \<tau> (X \<tau>)) on U(X t\<^sub>0)) \<Longrightarrow> D (\<lambda>\<tau>. \<mu>(X \<tau>)-\<nu>(X \<tau>)) = (\<lambda>\<tau>. \<mu>'(X \<tau>)-\<nu>'(X \<tau>)) on U(X t\<^sub>0)"
-  shows "diff_inv (\<lambda>s. \<nu> s \<le> \<mu> s) f U S t\<^sub>0 G"
+  shows "diff_inv U S G f t\<^sub>0 (\<lambda>s. \<nu> s \<le> \<mu> s)"
 proof(simp_all add: diff_inv_eq ivp_sols_def, safe)
   fix X t assume Ghyp: "\<forall>\<tau>. \<tau> \<in> U (X t\<^sub>0) \<and> \<tau> \<le> t \<longrightarrow> G (X \<tau>)"
   assume xivp: "D X = (\<lambda>x. f x (X x)) on U (X t\<^sub>0)" "\<nu> (X t\<^sub>0) \<le> \<mu> (X t\<^sub>0)" "X \<in> U (X t\<^sub>0) \<rightarrow> S"
@@ -191,7 +191,7 @@ lemma diff_inv_less_rule [diff_inv_rules]:
     and Gg: "\<And>X. (D X = (\<lambda>\<tau>. f \<tau> (X \<tau>)) on U(X t\<^sub>0)) \<Longrightarrow> (\<forall>\<tau>\<in>U(X t\<^sub>0). \<tau> > t\<^sub>0 \<longrightarrow> G (X \<tau>) \<longrightarrow> \<mu>' (X \<tau>) \<ge> \<nu>' (X \<tau>))"
     and Gl: "\<And>X. (D X = (\<lambda>\<tau>. f \<tau> (X \<tau>)) on U(X t\<^sub>0)) \<Longrightarrow> (\<forall>\<tau>\<in>U(X t\<^sub>0). \<tau> < t\<^sub>0 \<longrightarrow> \<mu>' (X \<tau>) \<le> \<nu>' (X \<tau>))"
     and dX: "\<And>X. (D X = (\<lambda>\<tau>. f \<tau> (X \<tau>)) on U(X t\<^sub>0)) \<Longrightarrow> D (\<lambda>\<tau>. \<mu>(X \<tau>)-\<nu>(X \<tau>)) = (\<lambda>\<tau>. \<mu>'(X \<tau>)-\<nu>'(X \<tau>)) on U(X t\<^sub>0)"
-  shows "diff_inv (\<lambda>s. \<nu> s < \<mu> s) f U S t\<^sub>0 G"
+  shows "diff_inv U S G f t\<^sub>0 (\<lambda>s. \<nu> s < \<mu> s)"
 proof(simp_all add: diff_inv_eq ivp_sols_def, safe)
   fix X t assume Ghyp: "\<forall>\<tau>. \<tau> \<in> U (X t\<^sub>0) \<and> \<tau> \<le> t \<longrightarrow> G (X \<tau>)"
   assume xivp: "D X = (\<lambda>x. f x (X x)) on U (X t\<^sub>0)" "\<nu> (X t\<^sub>0) < \<mu> (X t\<^sub>0)" "X \<in> U (X t\<^sub>0) \<rightarrow> S"
@@ -227,15 +227,15 @@ qed
 
 lemma diff_inv_nleq_rule:
   fixes \<mu>::"'a::banach \<Rightarrow> real"
-  shows "diff_inv (\<lambda>s. \<not> \<nu> s \<le> \<mu> s) f U S t\<^sub>0 G \<longleftrightarrow> diff_inv (\<lambda>s. \<nu> s > \<mu> s) f U S t\<^sub>0 G"
+  shows "diff_inv U S G f t\<^sub>0 (\<lambda>s. \<not> \<nu> s \<le> \<mu> s) \<longleftrightarrow> diff_inv U S G f t\<^sub>0 (\<lambda>s. \<nu> s > \<mu> s)"
   unfolding diff_inv_eq apply safe
   by (clarsimp, erule_tac x=s in allE, simp, erule_tac x=X in ballE, force, force)+
 
 lemma diff_inv_neq_rule [diff_inv_rules]:
   fixes \<mu>::"'a::banach \<Rightarrow> real"
-  assumes "diff_inv (\<lambda>s. \<nu> s < \<mu> s) f U S t\<^sub>0 G"
-    and "diff_inv (\<lambda>s. \<nu> s > \<mu> s) f U S t\<^sub>0 G"
-  shows "diff_inv (\<lambda>s. \<nu> s \<noteq> \<mu> s) f U S t\<^sub>0 G"
+  assumes "diff_inv U S G f t\<^sub>0 (\<lambda>s. \<nu> s < \<mu> s)"
+    and "diff_inv U S G f t\<^sub>0 (\<lambda>s. \<nu> s > \<mu> s)"
+  shows "diff_inv U S G f t\<^sub>0 (\<lambda>s. \<nu> s \<noteq> \<mu> s)"
 proof(unfold diff_inv_eq, clarsimp)
   fix s::'a and X::"real \<Rightarrow> 'a" and t::real
   assume "\<nu> s \<noteq> \<mu> s" and Xhyp: "X \<in> Sols U S f t\<^sub>0 s" 
@@ -255,8 +255,8 @@ lemma diff_inv_neq_rule_converse:
   assumes Uhyp: "\<And>s. s \<in> S \<Longrightarrow> is_interval (U s)" "\<And>s t. s \<in> S \<Longrightarrow> t \<in> U s \<Longrightarrow> t\<^sub>0 \<le> t"
     and conts: "\<And>X. (D X = (\<lambda>\<tau>. f \<tau> (X \<tau>)) on U(X t\<^sub>0)) \<Longrightarrow> continuous_on (\<P> X (U (X t\<^sub>0))) \<nu>"
       "\<And>X. (D X = (\<lambda>\<tau>. f \<tau> (X \<tau>)) on U(X t\<^sub>0)) \<Longrightarrow> continuous_on (\<P> X (U (X t\<^sub>0))) \<mu>"
-    and dI:"diff_inv (\<lambda>s. \<nu> s \<noteq> \<mu> s) f U S t\<^sub>0 G"
-  shows "diff_inv (\<lambda>s. \<nu> s < \<mu> s) f U S t\<^sub>0 G"
+    and dI:"diff_inv U S G f t\<^sub>0 (\<lambda>s. \<nu> s \<noteq> \<mu> s)"
+  shows "diff_inv U S G f t\<^sub>0 (\<lambda>s. \<nu> s < \<mu> s)"
 proof(unfold diff_inv_eq ivp_sols_def, clarsimp)
   fix X t assume Ghyp: "\<forall>\<tau>. \<tau> \<in> U (X t\<^sub>0) \<and> \<tau> \<le> t \<longrightarrow> G (X \<tau>)"
   assume xivp: "D X = (\<lambda>x. f x (X x)) on U (X t\<^sub>0)" "\<nu> (X t\<^sub>0) < \<mu> (X t\<^sub>0)" "X \<in> U (X t\<^sub>0) \<rightarrow> S"
@@ -290,15 +290,15 @@ proof(unfold diff_inv_eq ivp_sols_def, clarsimp)
 qed
 
 lemma diff_inv_conj_rule [diff_inv_rules]:
-  assumes "diff_inv I\<^sub>1 f U S t\<^sub>0 G"
-    and "diff_inv I\<^sub>2 f U S t\<^sub>0 G"
-  shows "diff_inv (\<lambda>s. I\<^sub>1 s \<and> I\<^sub>2 s) f U S t\<^sub>0 G"
+  assumes "diff_inv U S G f t\<^sub>0 I\<^sub>1"
+    and "diff_inv U S G f t\<^sub>0 I\<^sub>2"
+  shows "diff_inv U S G f t\<^sub>0 (\<lambda>s. I\<^sub>1 s \<and> I\<^sub>2 s)"
   using assms unfolding diff_inv_def by auto
 
 lemma diff_inv_disj_rule [diff_inv_rules]:
-  assumes "diff_inv I\<^sub>1 f U S t\<^sub>0 G"
-    and "diff_inv I\<^sub>2 f U S t\<^sub>0 G"
-  shows "diff_inv (\<lambda>s. I\<^sub>1 s \<or> I\<^sub>2 s) f U S t\<^sub>0 G"
+  assumes "diff_inv U S G f t\<^sub>0 I\<^sub>1"
+    and "diff_inv U S G f t\<^sub>0 I\<^sub>2"
+  shows "diff_inv U S G f t\<^sub>0 (\<lambda>s. I\<^sub>1 s \<or> I\<^sub>2 s)"
   using assms unfolding diff_inv_def by auto
 
 subsection \<open> Picard-Lindeloef \<close>
